---
title: 'f(rad A) âŠ† rad B?'
date: 2023-05-20
permalink: /posts/2023/05/blog-post-1/
tags:
  - algebra
---

While reading [Elements of the Representation Theory of Associative Algebras](https://www.cambridge.org/core/books/elements-of-the-representation-theory-of-associative-algebras/AA8066B5809D0F556A540400AD3A419C) by Andrzej Skowronski, Daniel Simson, and Ibrahim Assem, I came across a mistake in **Exercise 1, Chapter I**. 

The exercise is posed as follows:
> Let $$f : A \rightarrow B$$ be a homomorphism of $$K$$-algebras. Prove that $$f(\text{rad } A) \subseteq \text{rad } B$$.

However, the statement is incorrect.

## One simple counterexample

Consider the algebras $$ A := \mathbb{T}_2(K) = \begin{bmatrix} K & 0 \\ K & K \end{bmatrix}$$ and $$B := \mathbb{M}_2(K) = \begin{bmatrix} K & K \\ K & K \end{bmatrix}$$, with the canonical inclusion map $$f : A \hookrightarrow B$$.

First, observe that $$\text{rad } A = \begin{bmatrix} 0 & 0 \\ K & 0 \end{bmatrix}$$. This is because $$I := \begin{bmatrix} 0 & 0 \\ K & 0 \end{bmatrix}$$ is a two-sided nilpotent ideal of $$A$$, and $$A/I \cong \begin{bmatrix} K & 0 \\ 0 & K \end{bmatrix} \cong K \times K$$, implying by Corollary 1.4(c) that $$\text{rad } A = I$$. Next, $$\text{rad } B = 0$$ by the definition of the Jacobson radical, or alternatively, by a direct application of the Wedderburn-Artin theorem, as stated in Theorem 3.4. Thus, $$f(\text{rad } A) \not\subseteq \text{rad } B$$.

## Sufficient condition for correctness

We can add the condition that $$f$$ is surjective for the statement to hold true:

> Let $$f : A \rightarrow B$$ be a **surjective** homomorphism of $$K$$-algebras. Then $$f(\text{rad } A) \subseteq \text{rad } B$$.

Indeed, let $$b' \in f(\text{rad } A)$$, and let $$a' \in \text{rad } A$$ be such that $$b' = f(a')$$. We need to prove that $$b' \in \text{rad } B$$. By Lemma 1.3, it suffices to show that for any $$b \in B$$, the element $$1-b'b$$ has a right inverse. Let $$b \in B$$. Since $$f$$ is surjective, there exists $$a \in A$$ such that $$b = f(a)$$. Thus, we have: 

$$
\begin{split}
1-b'b = 1-f(a')f(a) = f(1-a'a).\\
\end{split}
$$

Since $$a' \in \text{rad } A$$, by Lemma 1.3, there exists $$r \in A$$ such that $$(1-a'a)r = 1$$. Therefore, $$f(r)$$ is a right inverse of $$1-b'b$$ in $$B$$, as:

$$
\begin{split}
(1-b'b)f(r) = f(1-a'a)f(r) = f((1-a'a)r) = f(1) = 1.\\
\end{split}
$$ 

Thus, $$b' \in \text{rad } B$$, completing the proof.

<!-- $$
\begin{split}
x & = \int_{\tau_0}^{\tau_n}\tau^{-\alpha}\; d\tau \\
  & = \frac{\tau_0^{1-\alpha}-\tau_n^{1-\alpha}}{a-1}
\end{split}
$$ -->